veric/semax_conseq.v
@@ -77,15 +77,15 @@ Qed.
 
 Lemma semax'_conseq {CS: compspecs}:
  forall E Delta P' (R': ret_assert) (P: assert) c (R: ret_assert),
-   (□ local (typecheck_environ Delta) ∗ (<affine> ⎡allp_fun_id Delta⎤ ∗ P) ⊢
+   (□ local (typecheck_environ Delta) ∗ (allp_fun_id Delta ∗ P) ⊢
                    (|={E}=> P')) ->
-   (□ local (typecheck_environ Delta) ∗ (<affine> ⎡allp_fun_id Delta⎤ ∗ RA_normal R') ⊢
+   (□ local (typecheck_environ Delta) ∗ (<affine> allp_fun_id Delta ∗ RA_normal R') ⊢
                    (|={E}=> RA_normal R)) ->
-   (□ local (typecheck_environ Delta) ∗ (<affine> ⎡allp_fun_id Delta⎤ ∗ RA_break R') ⊢
+   (□ local (typecheck_environ Delta) ∗ (<affine> allp_fun_id Delta ∗ RA_break R') ⊢
                    (|={E}=> RA_break R)) ->
-   (□ local (typecheck_environ Delta) ∗ (<affine> ⎡allp_fun_id Delta⎤ ∗ RA_continue R') ⊢
+   (□ local (typecheck_environ Delta) ∗ (<affine> allp_fun_id Delta ∗ RA_continue R') ⊢
                    (|={E}=> RA_continue R)) ->
-   (forall vl, □ local (typecheck_environ Delta) ∗ (<affine> ⎡allp_fun_id Delta⎤ ∗ RA_return R' vl) ⊢
+   (forall vl, □ local (typecheck_environ Delta) ∗ (<affine> allp_fun_id Delta ∗ RA_return R' vl) ⊢
                    (|={E}=> RA_return R vl)) ->
    semax' OK_spec E Delta P' c R' ⊢ semax' OK_spec E Delta P c R.
 Proof.
@@ -133,15 +133,15 @@ Qed.
 
 Lemma semax_conseq {CS: compspecs}:
  forall E Delta P' (R': ret_assert) P c (R: ret_assert) ,
-   (□ local (typecheck_environ Delta) ∗ (<affine> ⎡allp_fun_id Delta⎤ ∗ P) ⊢
+   (□ local (typecheck_environ Delta) ∗ (<affine> allp_fun_id Delta ∗ P) ⊢
                    (|={E}=> P') ) ->
-   (□ local (typecheck_environ Delta) ∗ (<affine> ⎡allp_fun_id Delta⎤ ∗ RA_normal R') ⊢
+   (□ local (typecheck_environ Delta) ∗ (<affine> allp_fun_id Delta ∗ RA_normal R') ⊢
                    (|={E}=> RA_normal R)) ->
-   (□ local (typecheck_environ Delta) ∗ (<affine> ⎡allp_fun_id Delta⎤ ∗ RA_break R') ⊢
+   (□ local (typecheck_environ Delta) ∗ (<affine> allp_fun_id Delta ∗ RA_break R') ⊢
                    (|={E}=> RA_break R)) ->
-   (□ local (typecheck_environ Delta) ∗ (<affine> ⎡allp_fun_id Delta⎤ ∗ RA_continue R') ⊢
+   (□ local (typecheck_environ Delta) ∗ (<affine> allp_fun_id Delta ∗ RA_continue R') ⊢
                    (|={E}=> RA_continue R)) ->
-   (forall vl, □ local (typecheck_environ Delta) ∗ (<affine> ⎡allp_fun_id Delta⎤ ∗ RA_return R' vl) ⊢
+   (forall vl, □ local (typecheck_environ Delta) ∗ (<affine> allp_fun_id Delta ∗ RA_return R' vl) ⊢
                    (|={E}=> RA_return R vl)) ->
    semax OK_spec E Delta P' c R' ->  semax OK_spec E Delta P c R.
 Proof.
@@ -380,12 +380,12 @@ Proof.
 Qed.
 
 Lemma semax_adapt_frame {cs} E Delta c (P P': assert) (Q Q' : ret_assert)
-   (H: □ local (typecheck_environ Delta) ∗ (<affine> ⎡allp_fun_id Delta⎤ ∗ P) ⊢
+   (H: □ local (typecheck_environ Delta) ∗ (<affine> allp_fun_id Delta ∗ P) ⊢
                    ∃ F: mpred, (|={E}=> (P' ∗ ⎡F⎤) ∧
-                         ⌜□ local (tc_environ Delta) ∗ <affine> ⎡allp_fun_id Delta⎤ ∗ RA_normal (frame_ret_assert Q' ⎡F⎤) ⊢ |={E}=> RA_normal Q⌝ ∧
-                         ⌜□ local (tc_environ Delta) ∗ <affine> ⎡allp_fun_id Delta⎤ ∗ RA_break (frame_ret_assert Q' ⎡F⎤) ⊢ |={E}=> RA_break Q⌝ ∧
-                         ⌜□ local (tc_environ Delta) ∗ <affine> ⎡allp_fun_id Delta⎤ ∗ RA_continue (frame_ret_assert Q' ⎡F⎤) ⊢ |={E}=> RA_continue Q⌝ ∧
-                         ⌜forall vl, □ local (tc_environ Delta) ∗ <affine> ⎡allp_fun_id Delta⎤ ∗ RA_return (frame_ret_assert Q' ⎡F⎤) vl ⊢ |={E}=> RA_return Q vl⌝))
+                         ⌜□ local (tc_environ Delta) ∗ <affine> allp_fun_id Delta ∗ RA_normal (frame_ret_assert Q' ⎡F⎤) ⊢ |={E}=> RA_normal Q⌝ ∧
+                         ⌜□ local (tc_environ Delta) ∗ <affine> allp_fun_id Delta ∗ RA_break (frame_ret_assert Q' ⎡F⎤) ⊢ |={E}=> RA_break Q⌝ ∧
+                         ⌜□ local (tc_environ Delta) ∗ <affine> allp_fun_id Delta ∗ RA_continue (frame_ret_assert Q' ⎡F⎤) ⊢ |={E}=> RA_continue Q⌝ ∧
+                         ⌜forall vl, □ local (tc_environ Delta) ∗ <affine> allp_fun_id Delta ∗ RA_return (frame_ret_assert Q' ⎡F⎤) vl ⊢ |={E}=> RA_return Q vl⌝))
    (SEM: semax(CS := cs) OK_spec E Delta P' c Q'):
    semax OK_spec E Delta P c Q.
 Proof.
@@ -400,7 +400,7 @@ Proof.
 Qed.
 
 Lemma semax_adapt_frame' {cs} E Delta c (P P': assert) (Q Q' : ret_assert)
-   (H: □ local (typecheck_environ Delta) ∗ (<affine> ⎡allp_fun_id Delta⎤ ∗ P) ⊢
+   (H: □ local (typecheck_environ Delta) ∗ (<affine> allp_fun_id Delta ∗ P) ⊢
                    ∃ F: mpred, (|={E}=> (P' ∗ ⎡F⎤) ∧
                          ⌜RA_normal (frame_ret_assert Q' ⎡F⎤) ⊢ |={E}=> RA_normal Q⌝ ∧
                          ⌜RA_break (frame_ret_assert Q' ⎡F⎤) ⊢ |={E}=> RA_break Q⌝ ∧
@@ -420,7 +420,7 @@ Proof.
 Qed.
 
 Lemma semax_adapt {cs} E Delta c (P P': assert) (Q Q' : ret_assert)
-   (H: □ local (typecheck_environ Delta) ∗ (<affine> ⎡allp_fun_id Delta⎤ ∗ P) ⊢
+   (H: □ local (typecheck_environ Delta) ∗ (<affine> allp_fun_id Delta ∗ P) ⊢
                    (|={E}=> P' ∧
                         ⌜RA_normal Q' ⊢ |={E}=> RA_normal Q⌝ ∧
                         ⌜RA_break Q' ⊢ |={E}=> RA_break Q⌝ ∧
